src/Classical.v
@@ -1,0 +1,181 @@
+(* Copyright 2022 Centrum Wiskunde & Informatica *)
+
+(* ON SEPERATION LOGIC *)
+(* Author: Hans-Dieter A. Hiep *)
+
+Require Import FunctionalExtensionality.
+Require Import PropExtensionality.
+Require Import List.
+Require Import ZArith.
+
+Require Import OnSeparationLogic.Heap.
+Require Import OnSeparationLogic.Language.
+
+Module Classical (Export HS: HeapSig).
+
+Module L := Language HS.
+Include L.
+
+Fixpoint satisfy (h: heap) (s: store) (p: assert): Prop :=
+  match p with
+  | test g => gval g s = true
+  | hasval e e' => dom h (e s) /\ h (e s) = e' s
+  | land p q => satisfy h s p /\ satisfy h s q
+  | lor p q => ~(~satisfy h s p /\ ~satisfy h s q)
+  | limp p q => satisfy h s p -> satisfy h s q
+  | lforall x p => forall v, satisfy h (store_update s x v) p
+  | lexists x p => ~forall v, ~satisfy h (store_update s x v) p
+  | sand p q => ~forall h1 h2, ~(Partition h h1 h2 /\ satisfy h1 s p /\ satisfy h2 s q)
+  | simp p q => forall h'' h', Partition h'' h h' -> satisfy h' s p -> satisfy h'' s q
+  end.
+
+Proposition satisfy_stable (h: heap) (s: store) (p: assert):
+  ~~satisfy h s p -> satisfy h s p.
+generalize dependent s. generalize dependent h.
+induction p; intros h s; simpl.
+- intro. destruct (g s). reflexivity.
+  exfalso; apply H; intro; inversion H0.
+- intro. destruct (dom_dec h (e s)).
+  split. assumption.
+  destruct (h (e s)).
+  destruct (Z.eq_dec z (e0 s)).
+  rewrite e1. reflexivity.
+  exfalso. apply H. intro.
+  destruct H1. apply n. inversion H2. reflexivity.
+  exfalso. apply H. intro.
+  destruct H1. inversion H2.
+  exfalso. apply H. intro.
+  destruct H1. apply H0. assumption.
+- intro. split.
+  apply IHp1. intro; apply H. intro; destruct H1. apply H0; assumption.
+  apply IHp2. intro; apply H. intro; destruct H1. apply H0; assumption.
+- intro. intro. apply H. intro. destruct H0.
+  apply H1. split; assumption.
+- intro. intro. apply IHp2. intro. apply H. intro.
+  apply H1. apply H2. assumption.
+- intro. intro. apply H. intro.
+  apply H1. assumption.
+- intro. intro.
+  apply IHp. intro. apply H. intro.
+  specialize H1 with v0. apply H0. assumption.
+- intro. intro. apply H. intro. apply H1. apply H0.
+- intros. apply IHp2. intro. apply H. intro.
+  apply H2. eapply H3. apply H0. apply H1.
+Qed.
+
+(* emp <-> dom h = Empty_set Z *)
+
+(* poitnsto <-> dom h = Singleton Z (eval e s) /\
+      h (eval e s) = eval e' s *)
+
+Proposition satisfy_land (h: heap) (s: store) (p q: assert):
+  satisfy h s (land p q) <-> satisfy h s p /\ satisfy h s q.
+simpl; split; intro; auto.
+Qed.
+
+Proposition satisfy_limp (h: heap) (s: store) (p q: assert):
+  satisfy h s (limp p q) <-> (satisfy h s p -> satisfy h s q).
+simpl; split; intro; auto.
+Qed.
+
+Proposition satisfy_lnot (h: heap) (s: store) (p: assert):
+  satisfy h s (lnot p) <-> ~satisfy h s p.
+simpl; split; intro; intro.
+pose proof (H H0). inversion H1.
+exfalso. apply H. assumption.
+Qed.
+
+Proposition satisfy_lor_intro1 (h: heap) (s: store) (p q: assert):
+  satisfy h s p -> satisfy h s (lor p q).
+simpl; intro. intro. destruct H0. apply H0; assumption.
+Qed.
+
+Proposition satisfy_lor_intro2 (h: heap) (s: store) (p q: assert):
+  satisfy h s q -> satisfy h s (lor p q).
+simpl; intro. intro. destruct H0. apply H1; assumption.
+Qed.
+
+Proposition satisfy_lor_elim (h: heap) (s: store) (p q r: assert):
+  satisfy h s (lor p q) -> (satisfy h s p -> satisfy h s r) ->
+  (satisfy h s q -> satisfy h s r) -> satisfy h s r.
+simpl; intros.
+apply satisfy_stable. intro.
+apply H. split.
+intro. apply H0 in H3. apply H2; assumption.
+intro. apply H1 in H3. apply H2; assumption.
+Qed.
+
+Proposition satisfy_p_lor_not_p (h: heap) (s: store) (p: assert):
+  satisfy h s (lor p (lnot p)).
+simpl. intro. destruct H.
+apply H0. intro. exfalso. apply H; assumption.
+Qed.
+
+Proposition satisfy_lforall (h: heap) (s: store) (x: V) (p: assert):
+  satisfy h s (lforall x p) <-> forall v, satisfy h (store_update s x v) p.
+simpl. tauto.
+Qed.
+
+Proposition satisfy_equals (h: heap) (s: store) (e0 e1: expr):
+  satisfy h s (equals e0 e1) <-> e0 s = e1 s.
+simpl. destruct (Z.eq_dec (eval e0 s) (eval e1 s)).
+rewrite e. tauto. split. intro. inversion H.
+intro. exfalso. apply n. assumption.
+Qed.
+
+Proposition satisfy_hasvaldash (h: heap) (s: store) (x: V):
+  satisfy h s (hasvaldash x) <-> dom h (s x).
+split; intro.
+- unfold hasvaldash in H.
+  remember (fresh (evar x)).
+  simpl in H.
+  destruct (dom_dec h (s x)). assumption.
+  exfalso.
+  apply H; clear H; intro; intro; destruct H.
+  rewrite store_update_lookup_same in H1.
+  rewrite store_update_lookup_diff in H1.
+  apply H0. apply dom_spec. rewrite H1. intro. inversion H2.
+  intro.
+  rewrite H2 in Heqv.
+  simpl in Heqv.
+  pose proof (fresh_notIn (x :: nil)).
+  rewrite <- Heqv in H3.
+  apply H3. left. reflexivity.
+- simpl. intro.
+  remember (h (s x)). destruct o.
+  specialize H0 with z.
+  apply H0; clear H0.
+  assert (store_update s (fresh (x :: nil)) z x = s x).
+  rewrite store_update_lookup_diff. reflexivity.
+  intro. pose proof (fresh_notIn (x :: nil)).
+  apply H1. rewrite H0. left. reflexivity.
+  rewrite H0.
+  rewrite store_update_lookup_same.
+  split; auto.
+  eapply dom_spec. apply H. symmetry; assumption.
+Qed.
+
+Definition validity (p: assert): Prop := forall h s, satisfy h s p.
+
+Definition strong_partial_correct (p: assert) (S: program) (q: assert) :=
+  forall h s, satisfy h s p ->
+    ~bigstep S (h, s) None /\
+    forall h' s', bigstep S (h, s) (Some (h', s')) -> satisfy h' s' q.
+
+Example out_of_memory (x: V) (e: expr):
+  strong_partial_correct (lforall x (hasvaldash x)) (new x e) false.
+unfold strong_partial_correct.
+intros.
+split.
+intro.
+inversion H0.
+intros.
+inversion H0.
+rewrite satisfy_lforall in H.
+specialize (H n).
+rewrite satisfy_hasvaldash in H.
+rewrite store_update_lookup_same in H.
+exfalso. apply H2. assumption.
+Qed.
+
+End Classical.
